GMAC spec change

code/experimental/gcm/Hacl.Spec.GMAC.fst
@@ -6,30 +6,42 @@ open Spec
 
 open FStar.Seq
 open FStar.Endianness
+open Hacl.Cast
+open Hacl.Spec.Endianness
+
+#set-options "--z3rlimit 30 --initial_fuel 0 --max_fuel 0 --initial_ifuel 0 --max_ifuel 0"
+
+(* Hacl types *)
+
+type sbytes = seq Hacl.UInt8.t
+type sword = w:sbytes{length w <= 16}
+type sword_16 = w:sbytes{length w = 16}
+type skey = sword_16
+type stag = sword_16
+
+let intro_sbytes (s:bytes) : GTot (s:sbytes) = seq_map uint8_to_sint8 s
 
 (* Pure GMAC state and function specs *)
 
 type gmac_state_ = | MkState: r:elem -> acc:elem -> pmsg:bytes{length pmsg < 16} -> gmac_state_
 
-#set-options "--z3rlimit 30 --initial_fuel 0 --max_fuel 0 --initial_ifuel 0 --max_ifuel 0"
-
 let gmac_alloc_spec : gmac_state_ = MkState zero zero createEmpty
 
-val gmac_init_spec: r:key -> GTot gmac_state_
-let gmac_init_spec r = MkState (encode r) zero createEmpty
+val gmac_init_spec: r:skey -> GTot gmac_state_
+let gmac_init_spec r = MkState (encode (reveal_sbytes r)) zero createEmpty
 
-val gmac_update_spec: st:gmac_state_ -> msg:bytes ->
+val gmac_update_spec: st:gmac_state_ -> msg:sbytes ->
   GTot (nst:gmac_state_{nst.r = st.r /\ length nst.pmsg = (length st.pmsg + length msg) % 16})
   (decreases (length msg))
 let rec gmac_update_spec st msg =
   if length msg + length st.pmsg >= 16 then begin
-    let block : word = st.pmsg @| (slice msg 0 (16 - length st.pmsg)) in
-    let nmsg : bytes = slice msg (16 - length st.pmsg) (length msg) in
+    let block : word = st.pmsg @| reveal_sbytes (slice msg 0 (16 - length st.pmsg)) in
+    let nmsg : sbytes = slice msg (16 - length st.pmsg) (length msg) in
     let nacc = (st.acc +@ (encode block)) *@ st.r in
     let nst = MkState st.r nacc createEmpty in
     gmac_update_spec nst nmsg
   end else begin
-    MkState st.r st.acc (st.pmsg @| msg)
+    MkState st.r st.acc (st.pmsg @| reveal_sbytes msg)
   end
 
 val gmac_last_spec: st:gmac_state_ -> GTot elem
@@ -37,23 +49,23 @@ let gmac_last_spec st =
   if length st.pmsg = 0 then st.acc
   else (st.acc +@ (encode st.pmsg)) *@ st.r
     
-val gmac_finish_spec: st:gmac_state_ -> s:tag ->
-  GTot (t:tag{t = finish (gmac_last_spec st) s})
+val gmac_finish_spec: st:gmac_state_ -> s:stag ->
+  GTot (t:tag{t = finish (gmac_last_spec st) (reveal_sbytes s)})
 let gmac_finish_spec st s = 
-  decode ((gmac_last_spec st) +@ (encode s))
+  decode ((gmac_last_spec st) +@ (encode (reveal_sbytes s)))
 
-val gmac_spec: msg:bytes -> r:key -> s:tag -> GTot tag
+val gmac_spec: msg:sbytes -> r:skey -> s:stag -> GTot tag
 let gmac_spec msg r s =
   let st_0 = gmac_init_spec r in
   let st = gmac_update_spec st_0 msg in
   gmac_finish_spec st s
   
-val flatten_bytes: msgs:seq bytes -> Tot bytes (decreases (length msgs))
-let rec flatten_bytes msgs =
+val flatten_sbytes: msgs:seq sbytes -> Tot sbytes (decreases (length msgs))
+let rec flatten_sbytes msgs =
   if length msgs = 0 then createEmpty
-  else (head msgs) @| (flatten_bytes (tail msgs))
+  else (head msgs) @| (flatten_sbytes (tail msgs))
   
-val gmac_update_spec_repeat: st:gmac_state_ -> msgs:seq bytes -> GTot gmac_state_ (decreases (length msgs))
+val gmac_update_spec_repeat: st:gmac_state_ -> msgs:seq sbytes -> GTot gmac_state_ (decreases (length msgs))
 let rec gmac_update_spec_repeat st msgs =
   if length msgs = 0 then st
   else
@@ -123,79 +135,83 @@ let rec lemma_encode_bytes msg_1 msg_2 =
     lemma_eq_intro (encode_bytes (msg_1 @| msg_2)) (cons msg_2 (encode_bytes msg_1))
   end
 
-val lemma_gmac_update_pmsg: st:gmac_state_ -> msg:bytes -> Lemma
+val lemma_gmac_update_pmsg: st:gmac_state_ -> msg:sbytes -> Lemma
   (requires True)
   (ensures (let st' = MkState st.r st.acc createEmpty in
-    gmac_update_spec st msg = gmac_update_spec st' (st.pmsg @| msg)))
+    gmac_update_spec st msg = gmac_update_spec st' (intro_sbytes st.pmsg @| msg)))
 let lemma_gmac_update_pmsg st msg =
   let st' = MkState st.r st.acc createEmpty in
   if length st.pmsg + length msg >= 16 then begin
-    let block : word = st.pmsg @| (slice msg 0 (16 - length st.pmsg)) in
-    let block' : word = createEmpty @| (slice (st.pmsg @| msg) 0 16) in
+    let block : word = st.pmsg @| reveal_sbytes (slice msg 0 (16 - length st.pmsg)) in
+    let block' : word = createEmpty @| reveal_sbytes (slice (intro_sbytes st.pmsg @| msg) 0 16) in
     lemma_eq_intro block block';
-    let nmsg : bytes = slice msg (16 - length st.pmsg) (length msg) in
-    let nmsg' : bytes = slice (st.pmsg @| msg) 16 (length st.pmsg + length msg) in
+    let nmsg : sbytes = slice msg (16 - length st.pmsg) (length msg) in
+    let nmsg' : sbytes = slice (intro_sbytes st.pmsg @| msg) 16 (length st.pmsg + length msg) in
     lemma_eq_intro nmsg nmsg'
-  end else lemma_eq_intro (createEmpty @| (st.pmsg @| msg)) (st.pmsg @| msg)
+  end else begin
+    lemma_eq_intro (createEmpty @| reveal_sbytes (intro_sbytes st.pmsg @| msg)) (st.pmsg @| reveal_sbytes msg)
+  end
 
-val lemma_gmac_update_0: st:gmac_state_{length st.pmsg = 0} -> msg_1:bytes -> msg_2:bytes -> Lemma
+val lemma_gmac_update_0: st:gmac_state_{length st.pmsg = 0} -> msg_1:sbytes -> msg_2:sbytes -> Lemma
   (requires True)
   (ensures (gmac_update_spec (gmac_update_spec st msg_1) msg_2 = gmac_update_spec st (msg_1 @| msg_2)))
   (decreases (length msg_1))
 let rec lemma_gmac_update_0 st msg_1 msg_2 =
   lemma_eq_intro st.pmsg createEmpty;
   if length msg_1 >= 16 then begin
-    let block : word = st.pmsg @| (slice msg_1 0 16) in
-    let block' : word = st.pmsg @| (slice (msg_1 @| msg_2) 0 16) in
+    let block : word = st.pmsg @| reveal_sbytes (slice msg_1 0 16) in
+    let block' : word = st.pmsg @| reveal_sbytes (slice (msg_1 @| msg_2) 0 16) in
     lemma_eq_intro block block';
-    let nmsg_1 : bytes = slice msg_1 16 (length msg_1) in
-    let nmsg' : bytes = slice (msg_1 @| msg_2) 16 (length msg_1 + length msg_2) in
+    let nmsg_1 : sbytes = slice msg_1 16 (length msg_1) in
+    let nmsg' : sbytes = slice (msg_1 @| msg_2) 16 (length msg_1 + length msg_2) in
     lemma_eq_intro (nmsg_1 @| msg_2) nmsg';
     let nacc = (st.acc +@ (encode block)) *@ st.r in
     let nst = MkState st.r nacc createEmpty in
     lemma_gmac_update_0 nst nmsg_1 msg_2
   end else begin 
-    let st' = MkState st.r st.acc msg_1 in
-    lemma_eq_intro (st.pmsg @| msg_1) msg_1;
+    let st' = MkState st.r st.acc (reveal_sbytes msg_1) in
+    lemma_eq_intro (st.pmsg @| reveal_sbytes msg_1) (reveal_sbytes msg_1);
+    lemma_eq_intro (intro_sbytes (reveal_sbytes msg_1)) msg_1;
     lemma_gmac_update_pmsg st' msg_2
   end
 
-val lemma_gmac_update_: st:gmac_state_ -> msg_1:bytes -> msg_2:bytes -> Lemma
+val lemma_gmac_update_: st:gmac_state_ -> msg_1:sbytes -> msg_2:sbytes -> Lemma
   (requires True)
   (ensures (gmac_update_spec (gmac_update_spec st msg_1) msg_2 = gmac_update_spec st (msg_1 @| msg_2)))
 let lemma_gmac_update_ st msg_1 msg_2 =
   let st' = MkState st.r st.acc createEmpty in
-  assert(length st'.pmsg = 0);
   lemma_gmac_update_pmsg st msg_1;
   lemma_gmac_update_pmsg st (msg_1 @| msg_2);
-  lemma_gmac_update_0 st' (st.pmsg @| msg_1) msg_2;
-  lemma_eq_intro ((st.pmsg @| msg_1) @| msg_2) (st.pmsg @| (msg_1 @| msg_2))
+  lemma_gmac_update_0 st' (intro_sbytes st.pmsg @| msg_1) msg_2;
+  append_assoc (intro_sbytes st.pmsg) msg_1 msg_2
 
 val lemma_gmac_update_empty: st:gmac_state_ -> Lemma (gmac_update_spec st createEmpty = st)
 let lemma_gmac_update_empty st = lemma_eq_intro (st.pmsg @| createEmpty) st.pmsg
 
 val lemma_gmac_update_last: st:gmac_state_{length st.pmsg = 0} ->
-  msg:bytes{length msg > 0 /\ length msg <= 16} -> Lemma
-  (gmac_last_spec (gmac_update_spec st msg) = (st.acc +@ (encode msg)) *@ st.r)
+  msg:sbytes{length msg > 0 /\ length msg <= 16} -> Lemma
+  (gmac_last_spec (gmac_update_spec st msg) = (st.acc +@ (encode (reveal_sbytes msg))) *@ st.r)
 let lemma_gmac_update_last st msg = 
   let st' = gmac_update_spec st msg in
   lemma_eq_intro st.pmsg createEmpty;
   if length msg = 16 then begin
-    let block : word = st.pmsg @| (slice msg 0 16) in
-    lemma_eq_intro block msg;
-    let nmsg : bytes = slice msg (16 - length st.pmsg) (length msg) in
+    let block : word = st.pmsg @| reveal_sbytes (slice msg 0 16) in
+    lemma_eq_intro block (reveal_sbytes msg);
+    let nmsg : sbytes = slice msg (16 - length st.pmsg) (length msg) in
     lemma_eq_intro nmsg createEmpty;
     let nacc = (st.acc +@ (encode block)) *@ st.r in
     let nst = MkState st.r nacc createEmpty in
     lemma_gmac_update_empty nst
-  end else lemma_eq_intro (st.pmsg @| msg) msg
+  end else begin
+    lemma_eq_intro (reveal_sbytes msg) (st.pmsg @| reveal_sbytes msg)
+  end
 
-val lemma_gmac_spec_short: msg:bytes{length msg < 16} -> r:key -> Lemma
+val lemma_gmac_spec_short: msg:sbytes{length msg < 16} -> r:skey -> Lemma
   (requires True)
   (ensures (
     let st_0 = gmac_init_spec r in
     let st = gmac_update_spec st_0 msg in
-    gmac_last_spec st = poly (encode_bytes msg) (encode r)))
+    gmac_last_spec st = poly (encode_bytes (reveal_sbytes msg)) (encode (reveal_sbytes r))))
 let lemma_gmac_spec_short msg r =
   let st_0 = gmac_init_spec r in
   let st = gmac_update_spec st_0 msg in
@@ -204,22 +220,22 @@ let lemma_gmac_spec_short msg r =
     lemma_eq_intro msg createEmpty
   end else begin
     lemma_eq_intro st_0.pmsg createEmpty;
-    lemma_eq_intro (st_0.pmsg @| msg) msg;
-    lemma_encode_bytes_0 createEmpty msg;
+    lemma_eq_intro (st_0.pmsg @| reveal_sbytes msg) (reveal_sbytes msg);
+    lemma_encode_bytes_0 createEmpty (reveal_sbytes msg);
     lemma_eq_intro (createEmpty @| msg) msg;
     lemma_eq_intro (encode_bytes createEmpty) createEmpty;
-    poly_cons msg (encode_bytes createEmpty) (encode r);
-    add_comm (encode msg) zero
+    poly_cons (reveal_sbytes msg) (encode_bytes createEmpty) (encode (reveal_sbytes r));
+    add_comm (encode (reveal_sbytes msg)) zero
   end
 
 #reset-options "--z3rlimit 20 --initial_fuel 0 --max_fuel 0 --initial_ifuel 0 --max_ifuel 0"
 
-val lemma_gmac_spec_: msg:bytes -> r:key -> Lemma
+val lemma_gmac_spec_: msg:sbytes -> r:skey -> Lemma
   (requires True)
   (ensures (
     let st_0 = gmac_init_spec r in
     let st = gmac_update_spec st_0 msg in
-    gmac_last_spec st = poly (encode_bytes msg) (encode r)))
+    gmac_last_spec st = poly (encode_bytes (reveal_sbytes msg)) (encode (reveal_sbytes r))))
   (decreases (length msg))
 let rec lemma_gmac_spec_ msg r = 
   let st_0 = gmac_init_spec r in
@@ -230,14 +246,14 @@ let rec lemma_gmac_spec_ msg r =
     let lhd = length msg - ltl in
     let hd, tl = split msg lhd in
     lemma_split msg lhd;
-    lemma_eq_intro msg (hd @| tl);
-    lemma_encode_bytes hd tl;
-    poly_cons tl (encode_bytes hd) (encode r);
+    lemma_eq_intro (reveal_sbytes msg) (reveal_sbytes hd @| reveal_sbytes tl);
+    lemma_encode_bytes (reveal_sbytes hd) (reveal_sbytes tl);
+    poly_cons (reveal_sbytes tl) (encode_bytes (reveal_sbytes hd)) (encode (reveal_sbytes r));
     lemma_gmac_spec_ hd r;
     lemma_gmac_update_ st_0 hd tl;
     let st' = gmac_update_spec st_0 hd in
     lemma_gmac_update_last st' tl;
-    add_comm (encode tl) (poly (encode_bytes hd) (encode r))
+    add_comm (encode (reveal_sbytes tl)) (poly (encode_bytes (reveal_sbytes hd)) (encode (reveal_sbytes r)))
   end
 
 
@@ -245,19 +261,20 @@ let rec lemma_gmac_spec_ msg r =
 
 #reset-options "--z3rlimit 20 --initial_fuel 1 --max_fuel 1 --initial_ifuel 0 --max_ifuel 0"
 
-val lemma_gmac_update: st:gmac_state_ -> msgs:seq bytes -> Lemma
+val lemma_gmac_update: st:gmac_state_ -> msgs:seq sbytes -> Lemma
   (requires True)
-  (ensures (gmac_update_spec_repeat st msgs = gmac_update_spec st (flatten_bytes msgs)))
+  (ensures (gmac_update_spec_repeat st msgs = gmac_update_spec st (flatten_sbytes msgs)))
   (decreases (length msgs))
 let rec lemma_gmac_update st msgs = 
   if length msgs = 0 then begin
     lemma_eq_intro st.pmsg (st.pmsg @| createEmpty)
   end else begin
     lemma_gmac_update (gmac_update_spec st (head msgs)) (tail msgs);
-    lemma_gmac_update_ st (head msgs) (flatten_bytes (tail msgs))
+    lemma_gmac_update_ st (head msgs) (flatten_sbytes (tail msgs))
   end
 
-val lemma_gmac_spec: msg:bytes -> r:key -> s:tag -> Lemma
+val lemma_gmac_spec: msg:sbytes -> r:skey -> s:stag -> Lemma
   (requires True)
-  (ensures (gmac_spec msg r s = mac (encode_bytes msg) (encode r) s))
+  (ensures (gmac_spec msg r s =
+    mac (encode_bytes (reveal_sbytes msg)) (encode (reveal_sbytes r)) (reveal_sbytes s)))
 let lemma_gmac_spec msg r s = lemma_gmac_spec_ msg r
