code/experimental/gcm/Hacl.Standalone.GMAC.fst
@@ -4,10 +4,10 @@ module U8   = FStar.UInt8
 module U32  = FStar.UInt32
 module H8   = Hacl.UInt8
 module H128 = Hacl.UInt128
-module Spec = Hacl.Spec.GMAC
 
-open Spec
 open Spec.GF128
+
+open Hacl.Spec.GMAC
 open Hacl.Impl.GF128
 
 open FStar.Mul
@@ -16,6 +16,8 @@ open FStar.Seq
 open FStar.Buffer
 open FStar.Endianness
 open Hacl.Endianness
+open Hacl.Spec.Endianness
+open Hacl.Cast
 
 #set-options "--z3rlimit 20 --initial_fuel 0 --max_fuel 0 --initial_ifuel 0 --max_ifuel 0"
 
@@ -37,11 +39,11 @@ let valid_st h (st:gmac_state) : Type0 =
   
 
 (* Get information from state *)
-  
-private let get_r h (st:gmac_state{valid_st h st}) : GTot elem =
-  sel_elem h (sub st.ram 0ul 1ul)
-private let get_acc h (st:gmac_state{valid_st h st}) : GTot elem =
-  sel_elem h (sub st.ram 1ul 1ul)
+
+private let get_len h (st:gmac_state{valid_st h st}) : GTot U32.t = get h st.len 0
+
+private let get_r h (st:gmac_state{valid_st h st}) : GTot elem = sel_elem h (sub st.ram 0ul 1ul)
+private let get_acc h (st:gmac_state{valid_st h st}) : GTot elem = sel_elem h (sub st.ram 1ul 1ul)
 private let get_pmsg h (st:gmac_state{valid_st h st}) :
   GTot (pmsg:bytes{Seq.length pmsg = U32.v (get h st.len 0)}) =
   decode_pmsg (get h st.ram 2) (get h st.len 0)
@@ -58,7 +60,7 @@ private let valid_pmsg_ (pmsg:H128.t) (len:U32.t) : Type0 =
   U32.v len < 16 /\ H128.v pmsg % (pow2 (8 * (16 - U32.v len))) = 0
 
 private val zero_div_mod: n:pos -> Lemma (0 / n = 0 /\ 0 % n = 0)
-let zero_div_mod n = ()
+let zero_div_mod n = Math.Lemmas.multiple_division_lemma 0 n; Math.Lemmas.multiple_modulo_lemma 0 n
 
 private val lemma_is_valid_pmsg_: pmsg:H128.t -> len:U32.t{valid_pmsg_ pmsg len} -> i:nat{i < 16 - U32.v len} ->
   Lemma (requires True)
@@ -86,11 +88,14 @@ let lemma_is_valid_pmsg pmsg len =
 
 val gmac_alloc: unit -> StackInline gmac_state
   (requires (fun _ -> True))
-  (ensures (fun h0 st h1 -> ~(contains h0 st.ram) /\
+  (ensures (fun h0 st h1 -> ~(contains h0 st.ram) /\ ~(contains h0 st.len) /\
     frameOf st.ram == h0.tip /\ frameOf st.len == h0.tip /\
     modifies_0 h0 h1 /\ valid_st h1 st))
 let gmac_alloc () =
+  let h0 = ST.get() in
   let ram = create zero_128 3ul in
+  let h1 = ST.get() in
+  lemma_reveal_modifies_0 h0 h1;
   let len = create 0ul 1ul in
   {ram = ram; len = len}
 
@@ -98,7 +103,7 @@ val gmac_init: st:gmac_state -> r:keyB{disjoint st.ram r /\ disjoint st.len r} -
   (requires (fun h -> valid_st h st /\ live h r))
   (ensures (fun h0 _ h1 -> valid_st h0 st /\ live h0 r /\ valid_st h1 st /\ live h1 r /\
     modifies_2 st.ram st.len h0 h1 /\
-    as_pure_st h1 st = gmac_init_spec (sel_word h0 r)))
+    as_pure_st h1 st = gmac_init_spec (as_seq h0 r)))
 let gmac_init st r =
   let h0 = ST.get() in
   let rv = encodeB r in
@@ -108,7 +113,7 @@ let gmac_init st r =
   st.len.(0ul) <- 0ul;
   let h1 = ST.get() in
   zero_div_mod (pow2 (8 * 16));
-  Seq.lemma_eq_intro (get_r h1 st) (encode (sel_word h0 r));
+  Seq.lemma_eq_intro (get_r h1 st) (encode (reveal_sbytes (as_seq h0 r)));
   fzero_lemma zero_128;
   Seq.lemma_eq_intro (get_acc h1 st) zero;
   Seq.lemma_eq_intro (get_pmsg h1 st) (Seq.createEmpty)
@@ -116,9 +121,37 @@ let gmac_init st r =
 private val update_pmsg: pmsg:H128.t -> len_1:U32.t{valid_pmsg_ pmsg len_1} ->
   nmsg:wordB -> len_2:U32.t{length nmsg = U32.v len_2 /\ U32.(v (len_1 +^ len_2)) <= 16} -> StackInline H128.t
   (requires (fun h -> live h nmsg))
-  (ensures (fun h0 r h1 -> h0 == h1 /\ live h0 nmsg /\ 
-    decode_pmsg r U32.(len_1 +^ len_2) = decode_pmsg pmsg len_1 @| sel_word h0 nmsg))
-let update_pmsg pmsg len_1 nmsg len_2 = admit()
+  (ensures (fun h0 r h1 -> live h0 nmsg /\ modifies_0 h0 h1 /\ valid_pmsg_ r U32.(len_1 +^ len_2) /\
+    decode_pmsg r U32.(len_1 +^ len_2) = decode_pmsg pmsg len_1 @| reveal_sbytes (as_seq h0 nmsg)))
+let update_pmsg pmsg len_1 nmsg len_2 =
+  let h0 = ST.get() in
+  push_frame();
+  let nmsg_16 = create (uint8_to_sint8 0uy) 16ul in
+  blit nmsg 0ul nmsg_16 len_1 len_2;
+  let h' = ST.get() in
+  let pmsg_ = encodeB nmsg_16 in
+  pop_frame();
+  let h1 = ST.get() in
+  lemma_eq_intro (slice ( (as_seq h' nmsg_16)) (U32.v len_1) (U32.v len_1 + U32.v len_2)) ( (as_seq h0 nmsg));
+  admit()
+  (*
+  admit();
+  lemma_eq_intro (sel_word h' nmsg_16) (pad (sel_word h' nmsg_16));
+  FStar.UInt.to_vec_lemma_2 (big_endian (sel_word h' nmsg_16)) (H128.v pmsg_);
+  assert(big_endian (sel_word h' nmsg_16) = H128.v pmsg_);
+  lemma_eq_intro (Seq.create (U32.v len_1) 0uy) (slice (sel_word h' nmsg_16) 0 (U32.v len_1));
+  admit();
+  lemma_eq_intro (Seq.create (U32.v len_1) 0uy @| slice (sel_word h' nmsg_16) (U32.v len_1) 16)
+    (sel_word h' nmsg_16);
+  admit();
+  *)
+  assume(H128.v pmsg + H128.v pmsg_ < pow2 128);
+  assume(valid_pmsg_ H128.(pmsg +^ pmsg_) U32.(len_1 +^ len_2));
+  assume(slice (decode_pmsg H128.(pmsg +^ pmsg_) U32.(len_1 +^ len_2)) 0 (U32.v len_1) = decode_pmsg pmsg len_1);
+  assume(slice (decode_pmsg H128.(pmsg +^ pmsg_) U32.(len_1 +^ len_2)) (U32.v len_1) (U32.v len_1 + U32.v len_2) = reveal_sbytes (as_seq h0 nmsg));
+  lemma_eq_intro (decode_pmsg H128.(pmsg +^ pmsg_) U32.(len_1 +^ len_2)) (decode_pmsg pmsg len_1 @| reveal_sbytes (as_seq h0 nmsg));
+  H128.(pmsg +^ pmsg_)
+  
 
 val gmac_update: st:gmac_state -> msg:buffer H8.t{disjoint st.ram msg /\ disjoint st.len msg} -> Stack unit
   (requires (fun h -> valid_st h st /\ live h msg))
